fix elpi test

theories/elpi_test.v
@@ -10,7 +10,7 @@ Variable u : Unif.
 Fixpoint of_goals l :=
   match l with
     | [::]%SEQ => [::]%G
-    | [:: hd & xs]%SEQ => [:: (hd, [::]) & of_goals xs]%G
+    | [:: hd & xs]%SEQ => [:: (hd.1, hd.2) & of_goals xs]%G
   end.
 
 Fixpoint of_alt l :=
@@ -19,8 +19,25 @@ Fixpoint of_alt l :=
   | [:: x & xs]%SEQ => (empty, of_goals x) ::: (of_alt xs)
   end.
 
+Definition clean_ca_G f (g : A * alts) :=
+  match g with
+  | (call a, ca) => (call a, [::])
+  | (cut, ca) => (cut, f ca)
+  end.
+
+Fixpoint clean_ca_goals gl :=
+  match gl with
+  | no_goals => nilC 
+  | more_goals hd tl => (clean_ca_G clean_ca hd) ::: (clean_ca_goals tl)
+  end
+with clean_ca (ats: alts) : alts :=
+  match ats with
+  | no_alt => nilC
+  | more_alt (hd,xs) tl => (hd, clean_ca_goals xs) ::: (clean_ca tl)
+  end.
+
 Definition tester l r :=
-  t2l l empty nilC = r.
+  clean_ca (t2l l empty nilC) = r.
 
 Goal forall B B0,
 let f x := (TA (call x)) in
@@ -31,6 +48,8 @@ Proof.
   by move=> //.
 Qed.
 
+Definition callN A := (call A, no_alt).
+
 Goal forall A B D0 D,
   (* (((! \/ A) \/ B)) /\ (D) *)
   let f x := (TA (call x)) in
@@ -38,9 +57,9 @@ Goal forall A B D0 D,
   tester 
     (And (Or ((Or (TA cut) empty (f A))) empty (f B)) (g D0) (f D)) 
     (of_alt [:: 
-      [:: (cut, of_alt [:: [:: (call B); (call D0)]]); (call D)];
-      [:: (call A); (call D0)]; 
-      [:: (call B); (call D0)]]).
+      [:: (cut, of_alt [:: [:: (callN B); (callN D0)]%SEQ]); (callN D)];
+      [:: (callN A); (callN D0)]; 
+      [:: (callN B); (callN D0)]]%SEQ).
 Proof.
   move=> A B D0 D p/=.
   move=>//=.
@@ -49,19 +68,20 @@ Qed.
 
 Goal forall B C D E F,
   let f x := (TA (call x)) in
-  let g x := ([::call x]) in
+  let g x := ([::call x]%SEQ) in
   (* (A \/_{empty} B) /\_C ((! \/_{empty} D) /\_{E} F) *)
   tester 
     (And (Or OK empty (f B)) (g C) (And (Or (TA cut) empty (f D)) (g E) (f F)))
     (of_alt [:: 
-      [:: cutE (of_alt [:: [:: callE B; callE C]]); callE F];
-      [:: callE D; callE E]; 
-      [:: callE B; callE C]]).
+      [:: (cut, (of_alt [:: [:: callN B; callN C]])); callN F];
+      [:: callN D; callN E]; 
+      [:: callN B; callN C]])%SEQ.
 Proof.
   move=> B C D E F p/=.
   rewrite //.
 Qed.
 
+Definition g x := ([::call x]%SEQ).
 (* THIS CAN NO MORE EXISTS: reset is never Bot *)
 (* Goal forall A B C,
   let f x := (TA (call x)) in
@@ -70,7 +90,7 @@ Qed.
     (And (Or ((Or (TA cut) empty (f A))) empty (f B)) Bot (Or (TA cut) empty (f C))) 
     (of_alt [:: 
       [::cut nilC ; cut nilC ];
-      [::cut nilC ; call p C]]).
+      [::cut nilC ; call p C]]%SEQ).
 Proof.
   move=> A B C p/=.
   rewrite/t2l//.
@@ -78,19 +98,17 @@ Qed. *)
 
 Goal forall A B C0 C,
   let f x := (TA (call x)) in
-  let g x := ([::call x]) in
+  let g x := ([::call x]%SEQ) in
   (* (((! \/ A) \/ B)) /\ (! \/ C)*)
   tester 
     (And (Or ((Or (TA cut) empty (f A))) empty (f B)) (g C0) (Or (TA cut) empty (f C)))
     (of_alt[:: 
-      [::cutE (of_alt [:: [:: callE B; callE C0]]); cutE (of_alt [::[:: callE A; callE C0]; [:: callE B; callE C0]])];
-      [::cutE (of_alt [:: [:: callE B; callE C0]]); callE C];
-      [:: callE A; callE C0]; 
-      [:: callE B; callE C0]]).
+      [::(cut, (of_alt [:: [:: callN B; callN C0]])); (cut, (of_alt [::[:: callN A; callN C0]; [:: callN B; callN C0]]))];
+      [::(cut, (of_alt [:: [:: callN B; callN C0]])); callN C];
+      [:: callN A; callN C0]; 
+      [:: callN B; callN C0]]%SEQ).
 Proof.
-  move=> A B C0 C p/=.
-  rewrite/t2l/=.
-  move=>//.
+  move=> A B C0 C p//=.
 Qed.
 
 
@@ -98,8 +116,8 @@ Qed.
 Goal forall A B0,
     (* (OK \/ A) /\_B0 OK *)
   let f x := (TA (call x)) in
-  let g x := ([::call x]) in
-  tester (And (Or OK empty (f A)) (g B0) OK) (of_alt [::[::]; [::callE A; callE B0]]).
+  let g x := ([::call x]%SEQ) in
+  tester (And (Or OK empty (f A)) (g B0) OK) (of_alt [::[::]; [::callN A; callN B0]]%SEQ).
 Proof.
   move=> A B0 p.
   rewrite/t2l//=.
@@ -108,9 +126,9 @@ Qed.
 Goal forall A B0,
   (* (Bot \/ B) /\_b0 B0  *)
   let f x := (TA (call x)) in
-  let g x := ([::call x]) in
+  let g x := ([::call x]%SEQ) in
   tester (And (Or Bot empty (f A)) (g B0) (f B0))
-  (of_alt [::[::callE A; callE B0]]).
+  (of_alt [::[::callN A; callN B0]]%SEQ).
 Proof.
   move=> A B0 p.
   rewrite/t2l//=.
@@ -118,14 +136,14 @@ Qed.
 
 Goal forall x y z w a, 
   let f x := (TA (call x)) in
-  let g x := ([::call x]) in
+  let g x := ([::call x]%SEQ) in
   tester (
     And 
       (Or (f x) empty (f y)) (g a) 
       (Or (f z) empty (f w))) 
-    (of_alt [:: [:: callE x; callE z];
-    [:: callE x; callE w];
-    [:: callE y; callE a]]).
+    (of_alt [:: [:: callN x; callN z];
+    [:: callN x; callN w];
+    [:: callN y; callN a]]%SEQ).
 Proof.
   move=>/=.
   by [].
@@ -133,12 +151,11 @@ Qed.
 
 Goal forall z w a, 
   let f x := (TA (call x)) in
-  let g x := ([::call x]) in
   tester (
     And 
       (Or OK empty Bot) (g a) 
       (Or (f z) empty (f w))) 
-    (of_alt [:: [:: callE z]; [:: callE w]]).
+    (of_alt [:: [:: callN z]; [:: callN w]]%SEQ).
 Proof.
   move=>p z w a.
   rewrite/t2l/=.
@@ -148,13 +165,12 @@ Qed.
 (* THIS IS IMPORTANT *)
 Goal forall a b c d, 
   let f x := (TA (call x)) in
-  let g x := ([::call x]) in
   tester (
     And 
       (Or Bot empty (f a)) (g b) 
       (Or (f c) empty (f d))) 
-    (* [:: [:: callE a; call b] ]. *)
-    (of_alt [:: [:: callE a; callE c]; [::callE a; callE d] ]).
+    (* [:: [:: callN a; call b] ]. *)
+    (of_alt [:: [:: callN a; callN c]; [::callN a; callN d] ]%SEQ).
 Proof.
   move=> a b c d /=.
   by [].
@@ -166,7 +182,7 @@ Goal forall a b,
     Or 
       (Or (TA cut) empty (TA (call a))) empty
       (TA (call b)))
-  (of_alt [:: [:: cutE (of_alt[:: [:: callE b]])]; [:: callE a]; [:: callE b]]).
+  (of_alt [:: [:: (cut, (of_alt[:: [:: callN b]]))]; [:: callN a]; [:: callN b]]%SEQ).
 Proof.
   move=> a b; rewrite/t2l/=.
   by []. Qed.
@@ -184,7 +200,7 @@ Qed. *)
 (* Goal forall A B C,
   let f x := (TA (call x)) in
   tester (And (Or (f A) empty (f B)) (Bot) (f C))
-  (of_alt[:: [:: callE A; call p C]]).
+  (of_alt[:: [:: callN A; call p C]]%SEQ).
 Proof.
   move=> s A B C p.
   rewrite/t2l/=.
@@ -193,33 +209,30 @@ Qed. *)
 
 Goal forall A1 A2 B0 C0 B,
   let f x := (TA (call x)) in
-  let g x := ([::call x]) in
   tester (And (Or (f A1) empty (f A2)) (g B0) (And Bot (g C0) (f B)))
-  (of_alt [:: [:: callE A2 ; callE B0 ]]).
+  (of_alt [:: [:: callN A2 ; callN B0 ]]%SEQ).
 Proof.
   move=> * /=.
   by [].
 Qed.
 
 Goal forall b0 a b c, 
-  let g x := ([::call x]) in
   tester (
     Or 
       (Or (And (TA (call c)) (g b0) (TA cut)) empty (TA (call a))) empty
       (TA (call b)))
-  (of_alt[:: [:: callE c; cutE (of_alt[:: [:: callE b]])]; [:: callE a]; [:: callE b]]).
+  (of_alt[:: [:: callN c; (cut, (of_alt[:: [:: callN b]]))]; [:: callN a]; [:: callN b]]%SEQ).
 Proof.
-  move=> b0 p a b c.
+  move=> b0 p a b .
   rewrite/t2l/=.
   rewrite//=.
 Qed.
 
 Goal forall B C Res,
   let f x := (TA (call x)) in
-  let g x := ([::call x]) in
   (* (OK \/ B) /\ (! \/ C) -> [cut_[B,Reset]; C; (B, Reset)] *)
   tester (And (Or OK empty (f B)) (g Res) (Or (TA cut) empty (f C))) 
-    (of_alt[::[::cutE (of_alt[::[:: callE B; callE Res]])]; [::callE C]; [:: callE B; callE Res]]).
+    (of_alt[::[::(cut, (of_alt[::[:: callN B; callN Res]]))]; [::callN C]; [:: callN B; callN Res]]%SEQ).
 Proof.
   move=> B C Res p.
   rewrite /t2l/=.
@@ -228,10 +241,9 @@ Qed.
 
 Goal forall B C Res Reempty,
   let f x := (TA (call x)) in
-  let g x := ([::call x]) in
   (* (OK \/ B) /\ (! /\ C) -> [cut_[]; C; (B, Reset)] *)
   tester (And (Or OK empty (f B)) (g Res) (And (TA cut) (g Reempty) (f C))) 
-    (of_alt[::[::cutE nilC; callE C]; [:: callE B; callE Res]]).
+    (of_alt[::[::(cut, nilC); callN C]; [:: callN B; callN Res]]%SEQ).
 Proof.
   move=> B C Res Reempty p/=.
   rewrite/t2l/=.
@@ -240,13 +252,12 @@ Qed.
 
 Goal forall A B C C0,
   let f x := (TA (call x)) in
-  let g x := ([::call x]) in
   (* (A /\ ((! \/ B) \/ C) *)
   tester (And (f A) (g C0) (Or (Or (TA cut) empty (f B)) empty (f C))) 
   (of_alt [:: 
-    [:: callE A; cutE (of_alt[:: [:: callE C]])]; 
-    [:: callE A; callE B]; 
-    [:: callE A; callE C]]).
+    [:: callN A; (cut, (of_alt[:: [:: callN C]]))]; 
+    [:: callN A; callN B]; 
+    [:: callN A; callN C]]%SEQ).
 Proof.
   move=> A B C C0 p.
   rewrite /t2l/=.
@@ -255,19 +266,16 @@ Qed.
 
 Goal forall A B C D E,
   let f x := (TA (call x)) in
-  let g x := ([::call x]) in
   (* (A \/_{empty} B) /\_C ((! \/_{empty} D) \/_{empty} E) *)
   tester 
     (And (Or (f A) empty (f B)) (g C) (Or (Or (TA cut) empty (f D)) empty (f E))) 
     (of_alt[:: 
-    [:: callE A; cutE (of_alt [:: [:: callE E]; [:: callE B; callE C]])];
-    [:: callE A; callE D]; [:: callE A; callE E];
-    [:: callE B; callE C]])
+    [:: callN A; (cut, (of_alt [:: [:: callN E]; [:: callN B; callN C]]))];
+    [:: callN A; callN D]; [:: callN A; callN E];
+    [:: callN B; callN C]]%SEQ)
   .
 Proof.
-  move=> empty A B C D E p/=.
-  rewrite/t2l/=.
-  move=>//.
+  by [].
 Qed.
 
 (* IMPORTANTE!
@@ -279,14 +287,13 @@ Qed.
 *)
 Goal forall B C D E,
   let f x := (TA (call x)) in
-  let g x := ([::call x]) in
   (* (OK \/_{empty} B) /\_C ((! \/_{empty} D) /\_{E} !) *)
   tester 
     (And (Or OK empty (f B)) (g C) (And (Or (TA cut) empty (f D)) (g E) (TA cut))) 
     (of_alt [:: 
-      [:: cutE (of_alt[:: [:: callE B; callE C]]); cutE nilC ];
-      [:: callE D; callE E]; 
-      [:: callE B; callE C]]).
+      [:: (cut, (of_alt[:: [:: callN B; callN C]])); (cut, nilC) ];
+      [:: callN D; callN E]; 
+      [:: callN B; callN C]]%SEQ).
 Proof.
   move=> B C D E p/=.
   rewrite/t2l/=.
@@ -299,11 +306,11 @@ Goal forall A B C,
   tester
     (Or (Or (Or (TA cut) empty ((Or (TA cut) empty (f A)))) empty (f B)) empty (f C))
     (of_alt[:: 
-      [::cutE (of_alt[:: [:: callE B]; [::callE C]])];
-      [::cutE (of_alt[:: [:: callE B]; [::callE C]])];
-      [:: callE A]; 
-      [:: callE B];
-      [:: callE C] ]).
+      [::(cut, (of_alt[:: [:: callN B]; [::callN C]]))];
+      [::(cut, (of_alt[:: [:: callN B]; [::callN C]]))];
+      [:: callN A]; 
+      [:: callN B];
+      [:: callN C] ]%SEQ).
 Proof.
   move=> A B C p/=.
   rewrite/t2l/=.
@@ -316,11 +323,11 @@ Goal forall A B C,
   tester 
     (Or (Or (Or (And (TA cut) ([::]) OK) empty ((Or (TA cut) empty (f A)))) empty (f B)) empty (f C)) 
     (of_alt[:: 
-      [::cutE (of_alt[:: [:: callE B]; [::callE C]])];
-      [::cutE (of_alt[:: [:: callE B]; [::callE C]])];
-      [:: callE A]; 
-      [:: callE B];
-      [:: callE C] ]).
+      [::(cut, (of_alt[:: [:: callN B]; [::callN C]]))];
+      [::(cut, (of_alt[:: [:: callN B]; [::callN C]]))];
+      [:: callN A]; 
+      [:: callN B];
+      [:: callN C] ]%SEQ).
 Proof.
   move=> A B C p/=.
   rewrite/t2l/=.
@@ -330,16 +337,15 @@ Qed.
 
 Goal forall A B C D0 D,
   let f x := (TA (call x)) in
-  let g x := ([::call x]) in
   (* (((! \/ ! \/ A) \/ B) \/ C) /\ D*)
   tester
     (And (Or (Or (Or (TA cut) empty ((Or (TA cut) empty (f A)))) empty (f B)) empty (f C)) (g D0) (f D))
     (of_alt[:: 
-      [::cutE (of_alt [:: [:: callE B; callE D0]; [::callE C; callE D0]]); callE D];
-      [::cutE (of_alt [:: [:: callE B; callE D0]; [::callE C; callE D0]]); callE D0];
-      [:: callE A; callE D0]; 
-      [:: callE B; callE D0];
-      [:: callE C; callE D0] ]).
+      [::(cut, (of_alt [:: [:: callN B; callN D0]; [::callN C; callN D0]])); callN D];
+      [::(cut, (of_alt [:: [:: callN B; callN D0]; [::callN C; callN D0]])); callN D0];
+      [:: callN A; callN D0]; 
+      [:: callN B; callN D0];
+      [:: callN C; callN D0] ]%SEQ).
 Proof.
   move=> A B C D0 D p/=.
   rewrite/t2l/=.
@@ -348,17 +354,16 @@ Qed.
 
 Goal forall X A B C D0 D,
   let f x := (TA (call x)) in
-  let g x := ([::call x]) in
   (* ((X \/ ((! \/ ! \/ A) \/ B) \/ C)) /\ D*)
   tester 
     (And (Or (f X) empty (Or (Or (Or (TA cut) empty ((Or (TA cut) empty (f A)))) empty (f B)) empty (f C))) (g D0) (f D))
     (of_alt[:: 
-      [:: callE X; callE D];
-      [::cutE (of_alt[:: [:: callE B; callE D0]; [::callE C; callE D0]]); callE D0];
-      [::cutE (of_alt[:: [:: callE B; callE D0]; [::callE C; callE D0]]); callE D0];
-      [:: callE A; callE D0]; 
-      [:: callE B; callE D0];
-      [:: callE C; callE D0] ]).
+      [:: callN X; callN D];
+      [::(cut, (of_alt[:: [:: callN B; callN D0]; [::callN C; callN D0]])); callN D0];
+      [::(cut, (of_alt[:: [:: callN B; callN D0]; [::callN C; callN D0]])); callN D0];
+      [:: callN A; callN D0]; 
+      [:: callN B; callN D0];
+      [:: callN C; callN D0] ]%SEQ).
 Proof.
   move=> X A B C D0 D p/=.
   rewrite/t2l/=.
@@ -367,14 +372,13 @@ Qed.
 
 Goal forall B0 A B C D,
   let f x := (TA (call x)) in
-  let g x := ([::call x]) in
   (* (((A /\ (! \/ B)) \/ C \/ D)) *)
   tester 
     (Or (Or (f C) empty (And (f A) (g B0) (Or (TA cut) empty (f B)))) empty (f D))
     (of_alt[:: 
-      [:: callE C]; 
-      [:: callE A; cutE (of_alt[:: [:: callE D]])]; 
-      [:: callE A; callE B]; [:: callE D]]).
+      [:: callN C]; 
+      [:: callN A; (cut, (of_alt[:: [:: callN D]]))]; 
+      [:: callN A; callN B]; [:: callN D]]%SEQ).
 Proof.
   move=> B0 A B C D p/=.
   rewrite/t2l/=.
@@ -387,12 +391,12 @@ Goal forall A B C,
   tester 
     (Or (Or (Or (Or (TA cut) empty (f A)) empty (TA cut)) empty (f B)) empty (f C))
     (of_alt[:: 
-      [::cutE (of_alt[::[::cutE (of_alt[::[::callE B]; [::callE C]])]; [::callE B]; [::callE C]])];
-      [::callE A];
-      [::cutE (of_alt[::[::callE B]; [::callE C]])];
-      [::callE B];
-      [::callE C]
-    ]).
+      [::(cut, (of_alt[::[::(cut, (of_alt[::[::callN B]; [::callN C]]))]; [::callN B]; [::callN C]]))];
+      [::callN A];
+      [::(cut, (of_alt[::[::callN B]; [::callN C]]))];
+      [::callN B];
+      [::callN C]
+    ]%SEQ).
 Proof.
   move=> p A B C/=.
   rewrite/t2l/=.
@@ -400,11 +404,12 @@ Proof.
 Qed.
 Goal forall p l,
   let s := ((Or (Or Dead empty (TA cut)) empty OK)) in
-  let bt := of_alt([::] :: l) in
-  t2l s empty (of_alt l) = of_alt[:: [:: cutE bt]; [::]] /\ 
+  let bt := of_alt([::]%SEQ :: l) in
+  t2l s empty (of_alt l) = of_alt[:: [:: (cut, bt)]; [::]]%SEQ /\ 
     t2l (odflt Bot (next_alt true (step u p empty s).2)) empty (of_alt l) ++ (of_alt l) = bt.
 Proof.
-  move=>//=.
+  move=>//= _ l.
+  rewrite cat_cons cat0s//.
 Qed.
 
 End Nur.
